sha/vst_lemmas.v
@@ -2,13 +2,78 @@
 
 Require Import VST.floyd.proofauto.
 Require Export sha.general_lemmas.
-Require Import sha.common_lemmas.
-Local Open Scope logic.
+
+Definition data_block {cs: compspecs} (sh: share) (contents: list byte) :=
+  @data_at cs sh (tarray tuchar (Zlength contents)) (map Vubyte contents).
+
+Lemma data_block_local_facts:
+ forall {cs: compspecs} sh f data,
+  data_block sh f data |--
+   prop (field_compatible (tarray tuchar (Zlength f)) [] data).
+Proof.
+intros. unfold data_block, array_at.
+simpl.
+entailer!.
+Qed.
+Hint Resolve @data_block_local_facts : saturate_local.
+
+
+Lemma data_block_valid_pointer {cs: compspecs} sh l p: sepalg.nonidentity sh -> Zlength l > 0 ->
+      data_block sh l p |-- valid_pointer p.
+Proof. unfold data_block. simpl; intros.
+  apply data_at_valid_ptr; auto; simpl.
+  rewrite Z.max_r, Z.mul_1_l; omega.
+Qed.
+
+Lemma split2_data_block:
+  forall  {cs: compspecs}  n sh data d,
+  (0 <= n <= Zlength data)%Z ->
+  data_block sh data d =
+  (data_block sh (sublist 0 n data) d *
+   data_block sh (sublist n (Zlength data) data)
+   (field_address0 (tarray tuchar (Zlength data)) [ArraySubsc n] d))%logic.
+Proof.
+  intros.
+  unfold data_block. simpl. normalize.
+  rewrite <- !sublist_map.
+  unfold tarray.
+  rewrite split2_data_at_Tarray_tuchar with (n1:=n) by (autorewrite with sublist; auto).
+  autorewrite with sublist.
+  reflexivity.
+Qed.
+
+Lemma split3_data_block:
+  forall  {cs: compspecs} lo hi sh data d,
+  0 <= lo <= hi ->
+  hi <= Zlength data  ->
+  data_block sh data d =
+  (data_block sh (sublist 0 lo data) d *
+   data_block sh (sublist lo hi data)
+   (field_address0 (tarray tuchar (Zlength data)) [ArraySubsc lo] d) *
+   data_block sh (sublist hi (Zlength data) data)
+   (field_address0 (tarray tuchar (Zlength data)) [ArraySubsc hi] d))%logic.
+Proof.
+  intros.
+  unfold data_block. 
+  rewrite <- !sublist_map.
+  unfold tarray.
+  rewrite split3_data_at_Tarray_tuchar with (n1:=lo)(n2:=hi) by (autorewrite with sublist; auto).
+  autorewrite with sublist.
+  reflexivity.
+Qed.
 
 Lemma force_lengthn_long {A}: forall n (l:list A) d, (n <= length l)%nat -> force_lengthn n l d = firstn n l.
 Proof. induction n; simpl; intros. trivial.
   destruct l; simpl in H. omega.
   rewrite IHn; trivial. omega.
+Qed.
+
+Lemma skipn_force_lengthn_app {A} n (l m:list A) a:
+        skipn n (force_lengthn n l a ++ m) = m.
+  intros. rewrite skipn_app1.
+  specialize (skipn_exact_length (force_lengthn n l a)).
+           rewrite force_lengthn_length_n. intros X; rewrite X; trivial.
+  rewrite force_lengthn_length_n; omega.
 Qed.
 
 Lemma data_at_triv {cs} sh t v v': v=v' -> @data_at cs sh t v |-- @data_at cs sh t v'.
@@ -17,53 +82,6 @@ Proof. intros; subst. auto. Qed.
 Lemma sizeof_Tarray {cs: composite_env} k: Z.max 0 k = k -> sizeof (Tarray tuchar k noattr) = k.
 Proof. intros K; simpl; rewrite K. destruct k; trivial. Qed.
 
-(*Require Import replace_refill_reptype_lemmas.*)
-(*
-Lemma data_at_Tarray_split3a {cs}: forall sh t n a i v,
-  0 <= i <= n ->
-  @data_at cs sh (Tarray t n a) v =
-  @data_at cs sh (Tarray t n a) (upd_Znth i v (Znth i v (default_val _))) v.
-    @data_at cs sh (Tarray t n a) (force_lengthn (nat_of_Z i) v (default_val _) ++
-      (Znth i v (default_val _)) :: skipn (nat_of_Z (i + 1)) v).
-Proof.
-  intros.
-  apply data_at_Tarray_ext.
-  intros j ?H.
-  unfold Znth.
-  if_tac; [omega |].
-  if_tac; [omega |].
-  unfold nat_of_Z.
-  destruct (Z_dec i j) as [[? | ?] | ?].
-  + assert ((Z.to_nat i < Z.to_nat j)%nat) by (apply Z2Nat.inj_lt in l; omega).
-    rewrite app_nth2 by (rewrite force_lengthn_length_n; omega).
-    rewrite force_lengthn_length_n.
-    simpl.
-    destruct ((Z.to_nat j - Z.to_nat i)%nat) eqn:?H; [omega |].
-    rewrite nth_skipn.
-    f_equal.
-    f_equal.
-    change (i + 1) with (Z.succ i).
-    rewrite Z2Nat.inj_succ by omega.
-    omega.
-  + assert ((Z.to_nat j < Z.to_nat i)%nat) by (apply Z2Nat.inj_lt; omega).
-    rewrite app_nth1 by (rewrite force_lengthn_length_n; omega).
-    rewrite nth_force_lengthn by omega.
-    reflexivity.
-  + subst.
-    rewrite app_nth2 by (rewrite force_lengthn_length_n; omega).
-    rewrite force_lengthn_length_n.
-    rewrite minus_diag.
-    simpl.
-    reflexivity.
-Qed.
-*)
-Lemma skipn_force_lengthn_app {A} n (l m:list A) a:
-        skipn n (force_lengthn n l a ++ m) = m.
-  intros. rewrite skipn_app1.
-  specialize (skipn_exact_length (force_lengthn n l a)).
-           rewrite force_lengthn_length_n. intros X; rewrite X; trivial.
-  rewrite force_lengthn_length_n; omega.
-Qed.
 
 Lemma sepcon_fold: forall Frame P rho,
 Frame = cons `(P) nil ->
@@ -105,159 +123,8 @@ apply Pos2Nat.inj_lt.
 apply H0.
 Qed.
 
-(*Same proof as semax_loadstore_array*)(*
-Lemma NEWsemax_loadstore_array:
-  forall {Espec: OracleKind},
- forall n k vi lo hi t1 (contents: Z -> reptype t1) v1 v2 (Delta: tycontext) e1 ei e2 sh P Q R,
-  (*H0*) reptype t1 = val ->
-  (*H1*) type_is_by_value t1 ->
-  (*H2*) legal_alignas_type t1 = true ->
-  (*H3*) typeof e1 = tarray t1 k->
-  (*H4*) typeof ei = tint ->
-  (*H8*) PROPx P (LOCALx Q (SEPx R)) |--  rel_expr e1 v1 && rel_expr ei (Vint (Int.repr vi))
-           && rel_expr (Ecast e2 t1) v2 ->
-  (*H7*) nth_error R n = Some (`(array_at t1 sh contents lo hi v1)) ->
-  (*H *) writable_share sh ->
-  (*H5*) tc_val t1 v2 ->
-  (*H6*) in_range lo hi vi ->
-   @semax Espec Delta (|> PROPx P (LOCALx Q (SEPx R))) (Sassign (Ederef (Ebinop Oadd e1 ei (tptr t1)) t1) e2)
-          (normal_ret_assert
-           (PROPx P (LOCALx Q (SEPx
-            (replace_nth n R `(array_at t1 sh (upd contents vi (valinject _ v2)) lo hi v1)))))).
-Proof.
-intros until R.
-intros H0 H1 H2 H3 H4 H8 H7 H H5 H6.
-eapply semax_post_flipped'.
-apply semax_loadstore_array'; eauto.
-apply derives_trans with (!! isptr v1 && PROPx P (LOCALx Q (SEPx R))).
-rewrite (SEP_nth_isolate _ _ _ H7).
-repeat rewrite <- insert_SEP.
-rewrite array_at_isptr. normalize.
-normalize.
-destruct v1; try contradiction.
-instantiate (2:=v1).
-simpl eval_binop. rewrite mul_repr.
-apply andp_right; auto.
-eapply derives_trans; [ apply H8 |].
-intro rho. simpl.
-repeat apply andp_right.
-apply rel_lvalue_deref.
-eapply rel_expr_binop.
-repeat apply andp_left1. apply derives_refl.
-apply andp_left1. apply andp_left2. apply derives_refl.
-intro; rewrite H4; simpl. rewrite H3; simpl.
-  unfold Cop.sem_add; simpl. rewrite mul_repr. auto.
- apply andp_left2. auto.
-rewrite (SEP_nth_isolate _ _ _ H7).
-repeat rewrite <- insert_SEP.
-apply derives_refl.
-rewrite (SEP_replace_nth_isolate _ _ _ `(array_at t1 sh (upd contents vi (valinject t1 v2)) lo hi v1) H7).
-rewrite insert_SEP.
-auto.
-Qed.*)
-(*
-Lemma array_at_local_facts':
-  forall (t : type) (sh : Share.t) (f : Z -> reptype t) (lo hi : Z) (v : val),
-  array_at t sh f lo hi v |-- array_at t sh f lo hi v && !!isptr v && !!offset_in_range (sizeof t * lo) v &&
-!!offset_in_range (sizeof t * hi) v && !!align_compatible t v.
-Proof. intros. unfold array_at. entailer. Qed.
-*)
-(*
-Lemma split_offset_array_at_: forall (ty : type) (sh : Share.t)
-         (z lo hi : Z) (v : val),
-       z <= lo <= hi ->
-       sizeof ty > 0 ->
-       legal_alignas_type ty = true ->
-       array_at_ ty sh z hi v =
-       !! offset_in_range (sizeof ty * z) v &&
-       !! offset_in_range (sizeof ty * hi) v &&
-       array_at_ ty sh z lo v *
-       array_at_ ty sh 0 (hi - lo)
-       (offset_val (Int.repr (sizeof ty * lo)) v).
-Proof.
-  intros. unfold array_at_.
-  rewrite <- split_offset_array_at; trivial.
-Qed.
-*)
-(*
-Lemma offset_val_array_at0:
- forall t sh f lo hi v,
-  sizeof t > 0 -> hi >= 0 ->
-  legal_alignas_type t = true ->
-  array_at t sh (fun i => f (i-lo)%Z) lo (lo + hi) v
-  |--
-  array_at t sh f 0 hi (offset_val (Int.repr (sizeof t * lo)) v).
-Proof.
-  intros.
-  rewrite (split_offset_array_at t _ _ lo lo); trivial.
-  rewrite array_at_emp.
-  entailer. rewrite Zplus_comm. rewrite Z.add_simpl_r.
-  apply array_lemmas.array_at_ext'. intros. rewrite Z.add_simpl_r. trivial.
-  omega.
-Qed.
-
-Lemma offset_val_array_at1:
- forall t sh f g k lo hi ofs v,
-    sizeof t > 0 -> hi >= 0 ->
-    legal_alignas_type t = true ->
-    k = lo + hi ->
-    g = (fun i => f (i-lo)%Z) ->
-    ofs = Int.repr (sizeof t * lo) ->
-  array_at t sh g lo k v |--
-  array_at t sh f 0 hi ((offset_val ofs) v).
-Proof.
-  intros. subst. apply offset_val_array_at0; trivial.
-Qed.
-*)
-(*
-Lemma split_memory_block p hi v sh:
-      0 <= p <= hi -> isptr v ->
-      memory_block sh (Int.repr hi) v =
-      !!offset_in_range (sizeof tuchar * 0) v &&
-      !!offset_in_range (sizeof tuchar * hi) v &&
-      memory_block sh (Int.repr p) v * memory_block sh (Int.repr (hi-p)) (offset_val (Int.repr p) v).
-Proof. intros.
-rewrite memory_block_array_tuchar'; try omega; trivial.
-rewrite memory_block_array_tuchar'; try omega; trivial.
-rewrite memory_block_array_tuchar'; try omega.
-rewrite (split_offset_array_at_ _ _ _ p).
-   assert (K: (sizeof tuchar * p = p)%Z).
-      assert (sizeof tuchar =1 ). reflexivity.
-  rewrite H1. omega.
-  rewrite K; trivial.
- assumption. simpl; omega. reflexivity. apply isptr_offset_val'; trivial.
-Qed.
-*)
 Lemma isptrD v: isptr v -> exists b ofs, v = Vptr b ofs.
 Proof. intros. destruct v; try contradiction. exists b, i; trivial. Qed.
-
-(*
-Lemma mysemax_frame_PQR:
-  forall R2 Espec Delta R1 P Q P' Q' R1' c,
-     closed_wrt_modvars c (LOCALx nil (SEPx R2)) ->
-     @semax Espec Delta (PROPx P (LOCALx Q (SEPx R1))) c
-                     (normal_ret_assert (PROPx P' (LOCALx Q' (SEPx R1')))) ->
-     @semax Espec Delta (PROPx P (LOCALx (Q) (SEPx (R1++R2)))) c
-                     (normal_ret_assert (PROPx P' (LOCALx (Q') (SEPx (R1'++R2))))).
-Proof.
-intros. specialize (semax_frame_PQR nil R2 Espec Delta R1 P Q P' Q' R1' c).
-repeat rewrite app_nil_r. intros. apply H1; trivial. Qed.
-
-Ltac frame_SEP'' L :=
- grab_indexes_SEP L;
- match goal with
- | |- @semax _ _ (PROPx _ (LOCALx _ (SEPx ?R))) _ _ =>
-  rewrite <- (firstn_skipn (length L) R);
-    simpl length; unfold firstn, skipn;
-    eapply (mysemax_frame_PQR);
-      [ unfold closed_wrt_modvars;  auto 50 with closed
-     | ]
- | |- (PROPx _ (LOCALx _ (SEPx ?R))) |-- _ =>
-  rewrite <- (firstn_skipn (length L) R);
-    simpl length; unfold firstn, skipn;
-    apply derives_frame_PQR
-end.
-*)
 
 Ltac myframe_SEP'' L :=  (* this should be generalized to permit framing on LOCAL part too *)
  grab_indexes_SEP L;
