sha/verif_hkdf.v
@@ -2,6 +2,7 @@ Require Import VST.floyd.proofauto.
 Import ListNotations.
 Local Open Scope logic.
 
+Require Import sha.vst_lemmas.
 Require Import sha.hmac_common_lemmas.
 
 Require Import sha.hkdf.
@@ -65,9 +66,9 @@ destruct (zlt 255 ((olen + 31) / 32)); inv EXPAND_RES.
    temp _salt_len (Vint (Int.repr (LEN SALT))); temp _secret secret;
    temp _secret_len (Vint (Int.repr (LEN SECRET))); temp _info info;
    temp _info_len (Vint (Int.repr (LEN INFO))); gvars gv)
-   SEP (spec_sha.K_vector gv; spec_sha.data_block Tsh (CONT INFO) info;
-   spec_sha.data_block Tsh (HKDF_extract (CONT SALT) (CONT SECRET)) v_prk;
-   memory_block shmd olen out; FRZL FR2; data_at Tsh tuint (Vint (Int.repr 32)) v_prk_len)).
+   SEP (spec_sha.K_vector gv; data_block Tsh (CONT INFO) info;
+        data_block Tsh (HKDF_extract (CONT SALT) (CONT SECRET)) v_prk;
+        memory_block shmd olen out; FRZL FR2; data_at Tsh tuint (Vint (Int.repr 32)) v_prk_len)).
   { congruence. }
   { forward. entailer!. }
 
@@ -76,7 +77,7 @@ destruct (zlt 255 ((olen + 31) / 32)); inv EXPAND_RES.
     thaw FR2. cancel. erewrite (split2_data_at__Tarray_tuchar Tsh 64 32); simpl; trivial; try omega.
     rewrite field_address_offset by auto with field_compatible. simpl.
     rewrite isptr_offset_val_zero; trivial. cancel.
-    unfold spec_sha.data_block. normalize. rewrite ZlengthExtract. cancel. }
+    unfold data_block. normalize. rewrite ZlengthExtract. cancel. }
   { discriminate. } 
   apply semax_ff.
 
@@ -87,9 +88,9 @@ destruct (zlt 255 ((olen + 31) / 32)); inv EXPAND_RES.
    temp _salt_len (Vint (Int.repr (LEN SALT))); temp _secret secret;
    temp _secret_len (Vint (Int.repr (LEN SECRET))); temp _info info;
    temp _info_len (Vint (Int.repr (LEN INFO))); gvars gv)
-   SEP (spec_sha.K_vector gv; spec_sha.data_block Tsh (CONT INFO) info;
-   spec_sha.data_block Tsh (HKDF_extract (CONT SALT) (CONT SECRET)) v_prk;
-   spec_sha.data_block shmd (HKDF_expand (HKDF_extract (CONT SALT) (CONT SECRET)) (CONT INFO) olen) out;
+   SEP (spec_sha.K_vector gv; data_block Tsh (CONT INFO) info;
+        data_block Tsh (HKDF_extract (CONT SALT) (CONT SECRET)) v_prk;
+        data_block shmd (HKDF_expand (HKDF_extract (CONT SALT) (CONT SECRET)) (CONT INFO) olen) out;
    FRZL FR2; data_at Tsh tuint (Vint (Int.repr 32)) v_prk_len))).
   { congruence. }
   { forward. entailer!. }
@@ -101,9 +102,9 @@ destruct (zlt 255 ((olen + 31) / 32)); inv EXPAND_RES.
    temp _salt salt; temp _salt_len (Vint (Int.repr (LEN SALT))); temp _secret secret;
    temp _secret_len (Vint (Int.repr (LEN SECRET))); temp _info info;
    temp _info_len (Vint (Int.repr (LEN INFO))); gvars gv)
-   SEP (spec_sha.K_vector gv; spec_sha.data_block Tsh (CONT INFO) info;
-   spec_sha.data_block Tsh (HKDF_extract (CONT SALT) (CONT SECRET)) v_prk;
-   spec_sha.data_block shmd (HKDF_expand (HKDF_extract (CONT SALT) (CONT SECRET)) (CONT INFO) olen) out;
+   SEP (spec_sha.K_vector gv; data_block Tsh (CONT INFO) info;
+        data_block Tsh (HKDF_extract (CONT SALT) (CONT SECRET)) v_prk;
+        data_block shmd (HKDF_expand (HKDF_extract (CONT SALT) (CONT SECRET)) (CONT INFO) olen) out;
    FRZL FR2; data_at Tsh tuint (Vint (Int.repr 32)) v_prk_len))).
   { elim H; trivial. }
   { clear H; forward. entailer!. }
@@ -111,5 +112,5 @@ destruct (zlt 255 ((olen + 31) / 32)); inv EXPAND_RES.
   erewrite (split2_data_at__Tarray_tuchar Tsh 64 32); simpl; trivial; try omega.
   rewrite field_address_offset by auto with field_compatible. simpl.
   rewrite isptr_offset_val_zero; trivial. cancel.
-  unfold spec_sha.data_block. normalize. rewrite ZlengthExtract. cancel.
+  unfold data_block. normalize. rewrite ZlengthExtract. cancel.
 Time Qed. (*Finished transaction in 2.151 secs (2.147u,0.003s) (successful)*)
